Semantics.thy
@@ -1,198 +1,522 @@
 theory Semantics
-  imports Structure "HOL-Library.Mapping"
+  imports "Definitions" "Registers" "Memory" "Partial_Function_MR/Partial_Function_MR"
 begin
 
-type_synonym register_state = "(llvm_identifier, llvm_value) mapping"
+section "Simps"
 
-datatype memory_entry = mem_unset | mem_value llvm_value | mem_freed
-type_synonym mem = "llvm_address \<rightharpoonup> memory_entry"
-
-definition disjoint :: "mem \<Rightarrow> mem \<Rightarrow> bool" where
-  "disjoint h1 h2 \<equiv> dom h1 \<inter> dom h2 = {}"
-
-definition union :: "mem \<Rightarrow> mem \<Rightarrow> mem" ("_ \<union> _" 50) where
-  "(h1 \<union> h2) \<equiv> h1 ++ h2"
-
-definition separating_conjunction :: "(mem \<Rightarrow> bool) \<Rightarrow> (mem \<Rightarrow> bool) \<Rightarrow> (mem \<Rightarrow> bool)" ("_ * _" 50) where
-  "(A * B) h \<equiv> (\<exists>h1 h2. disjoint h1 h2 \<and> h = union h1 h2 \<and> A h1 \<and> B h2)"
-
-definition valid :: "llvm_address \<Rightarrow> mem \<Rightarrow> bool" where
-  "valid l h \<equiv> dom h = {l} \<and> h \<noteq> [l \<mapsto> mem_freed]"
-
-definition contains :: "llvm_address \<Rightarrow> llvm_value \<Rightarrow> (mem \<Rightarrow> bool)" ("_ \<mapsto> _" 50) where
-  "(l \<mapsto> v) h \<equiv> h = [l \<mapsto> mem_value v]"
-
-definition empty :: "mem \<Rightarrow> bool" where
-  "empty h \<equiv> h = Map.empty"
-
-definition prop_empty :: "bool \<Rightarrow> mem \<Rightarrow> bool" where
-  "prop_empty P h \<equiv> empty h \<and> P"
-definition separating_implication :: "(mem \<Rightarrow> bool) \<Rightarrow> (mem \<Rightarrow> bool) \<Rightarrow> (mem \<Rightarrow> bool)" where
-  "separating_implication A B h \<equiv> (\<forall>h'. (disjoint h h' \<and> A h') \<longrightarrow> B (union h h'))"
-
-datatype state = state register_state mem
+lemma wp_case_value_addr_intro[wp_intro]:
+  assumes "\<And>x. a = addr x \<Longrightarrow> wp (f x) Q"
+  assumes "\<not>(\<exists>x. a = addr x) \<Longrightarrow> wp g Q"
+  shows "wp (case a of addr x \<Rightarrow> f x | _ \<Rightarrow> g) Q"
+  using assms
+  unfolding wp_def
+  by (cases "a"; auto)
 
 
 
-definition set_register :: "llvm_identifier \<Rightarrow> llvm_value \<Rightarrow> state \<Rightarrow> state" where
-  "set_register i v s = (case s of state r m \<Rightarrow> state (Mapping.update i v r) m)"
+section "Memory instructions"
 
-definition get_register :: "llvm_identifier \<Rightarrow> state \<Rightarrow> llvm_value option" where
-  "get_register i s = (case s of state r m \<Rightarrow> Mapping.lookup r i)"
+definition execute_alloca :: "llvm_identifier \<Rightarrow> state \<Rightarrow> state option" where
+  "execute_alloca name s = do {
+      (s', a) \<leftarrow> Some (allocate_stack s);
+      set_register name (addr a) s'
+    }"
 
+lemma alloca_wp_intro[THEN consequence, wp_intro]:
+  "wp (execute_alloca name s) (\<lambda>s'. \<exists>a. (register_\<alpha> s' = (register_\<alpha> s)(reg name := Some (addr a)) \<and> memory_\<alpha> s' = (memory_\<alpha> s)(a := Some None) \<and> memory_\<alpha> s a = None))"
+  unfolding execute_alloca_def
+  by (intro wp_intro; auto)
 
+thm alloca_wp_intro
 
-fun addr_index :: "llvm_address \<Rightarrow> nat" where
-  "addr_index (saddr n) = n"
-| "addr_index (haddr n) = n"
-
-fun is_saddr where
-  "is_saddr (saddr _) = True"
-| "is_saddr _ = False"
-
-fun is_haddr where
-  "is_haddr (haddr _) = True"
-| "is_haddr _ = False"
-
-definition max_address :: "llvm_address set \<Rightarrow> nat" where
-  "max_address d =
-     (if d = {} then 0 else Max (addr_index ` d))"
-
-definition fresh_stack_address :: "mem \<Rightarrow> llvm_address" where
-  "fresh_stack_address h =
-     (let saddrs = {a \<in> dom h. is_saddr a}
-      in saddr (Suc (max_address saddrs)))"
-
-definition fresh_heap_address :: "mem \<Rightarrow> llvm_address" where
-  "fresh_heap_address h =
-     (let haddrs = {a \<in> dom h. is_haddr a}
-      in haddr (Suc (max_address haddrs)))"
+lemma cons_ex:
+  assumes "wp c (\<lambda>s. \<exists>x. P x s)"
+  assumes "\<And>s x. P x s \<Longrightarrow> Q s"
+  shows "wp c Q"
+  oops
+  
 
 
-lemma mem_helper:
-  assumes "finite (dom h)"
-  and "haddr ad = fresh_heap_address h"
-  and "is_haddr x"
-  and "h x = Some y"
-  shows "addr_index x < ad"
-proof (-)
-  have "ad = Suc (if \<forall>x. x \<in> dom h \<longrightarrow> \<not> is_haddr x then 0 else Max (addr_index ` {a \<in> dom h. is_haddr a}))"
-    using assms
-    unfolding fresh_heap_address_def max_address_def
-    by simp
+fun get_address_from_pointer :: "state \<Rightarrow> llvm_pointer \<Rightarrow> llvm_address option" where
+  "get_address_from_pointer s p = do {
+    a \<leftarrow> get_register s p;
+    (case a of (addr a') \<Rightarrow> Some a' | _ \<Rightarrow> None)
+  }"
 
-  moreover
+definition execute_store :: "llvm_value_ref \<Rightarrow> llvm_pointer \<Rightarrow> state \<Rightarrow> state option" where
+  "execute_store v p s = do {
+    address \<leftarrow> get_address_from_pointer s p;
+    value \<leftarrow> get_register s v;
+    set_memory address value s
+  }"
 
-  obtain x' where xdef: "haddr x' = x"
-    using assms
-    by (cases x; simp)
-
-  then have "x' \<in> addr_index ` {a \<in> dom h. is_haddr a}"
-    using assms
-    by force
-
-  then have "x' \<le> Max (addr_index ` {a \<in> dom h. is_haddr a})"
-    using assms xdef by simp
-
-  then have "addr_index x \<le> (if \<forall>x. x \<in> dom h \<longrightarrow> \<not> is_haddr x then 0 else Max (addr_index ` {a \<in> dom h. is_haddr a}))"
-    using assms xdef by auto
-
-  ultimately
-
-  show ?thesis by simp
-qed
-
-lemma stack_helper:
-  assumes "finite (dom h)"
-  and "saddr ad = fresh_stack_address h"
-  and "is_saddr x"
-  and "h x = Some y"
-  shows "addr_index x < ad"
-proof (-)
-  have "ad = Suc (if \<forall>x. x \<in> dom h \<longrightarrow> \<not> is_saddr x then 0 else Max (addr_index ` {a \<in> dom h. is_saddr a}))"
-    using assms
-    unfolding fresh_stack_address_def max_address_def
-    by simp
-
-  moreover
-
-  obtain x' where xdef: "saddr x' = x"
-    using assms
-    by (cases x; simp)
-
-  then have "x' \<in> addr_index ` {a \<in> dom h. is_saddr a}"
-    using assms
-    by force
-
-  then have "x' \<le> Max (addr_index ` {a \<in> dom h. is_saddr a})"
-    using assms xdef by simp
-
-  then have "addr_index x \<le> (if \<forall>x. x \<in> dom h \<longrightarrow> \<not> is_saddr x then 0 else Max (addr_index ` {a \<in> dom h. is_saddr a}))"
-    using assms xdef by auto
-
-  ultimately
-
-  show ?thesis by simp
-qed
+lemma store_wp_intro[THEN consequence, wp_intro]:
+  assumes "register_\<alpha> s pointer = Some (addr a)" "memory_\<alpha> s a \<noteq> None"
+  assumes "register_\<alpha> s value = Some v"
+  shows "wp (execute_store value pointer s) (\<lambda>s'. memory_\<alpha> s' = (memory_\<alpha> s)(a := Some (Some v)) \<and> register_\<alpha> s' = register_\<alpha> s)"
+  unfolding execute_store_def
+  using assms
+  apply simp
+  by (intro wp_intro; auto)
 
 
-lemma fresh_heap_not_in_dom: "finite (dom h) \<Longrightarrow> fresh_heap_address h \<notin> dom h"
-  using mem_helper unfolding fresh_heap_address_def by force
+definition execute_load :: "llvm_identifier \<Rightarrow> llvm_pointer \<Rightarrow> state \<Rightarrow> state option" where
+  "execute_load n p s = do {
+    a \<leftarrow> get_address_from_pointer s p;
+    v \<leftarrow> get_memory s a;
+    set_register n v s
+  }"
 
-lemma fresh_stack_not_in_dom: "finite (dom h) \<Longrightarrow> fresh_stack_address h \<notin> dom h"
-  using stack_helper unfolding fresh_stack_address_def by force
-
-
-definition allocate_stack :: "state \<Rightarrow> (state * llvm_address)" where
-  "allocate_stack s \<equiv> (case s of state r m \<Rightarrow> (let a = fresh_stack_address m in (state r (m(a \<mapsto> mem_unset)), a)))"
-
-definition allocate_heap :: "state \<Rightarrow> (state * llvm_address)" where
-  "allocate_heap s \<equiv> (case s of state r m \<Rightarrow> (let a = fresh_heap_address m in (state r (m(a \<mapsto> mem_unset)), a)))"
-
-
-definition "get_memory a s \<equiv> (case s of state r m \<Rightarrow> (case m a of Some (mem_value v) \<Rightarrow> Some v | _ \<Rightarrow> None))"
-
-definition "set_memory a v s \<equiv> (case s of state r m \<Rightarrow> (case m a of None \<Rightarrow> None | Some mem_freed \<Rightarrow> None | _ \<Rightarrow> Some (state r (m(a := Some (mem_value v))))))"
-
-lemma "((a \<mapsto> v) * B) m \<Longrightarrow> get_memory a (state r m) = Some v"
-  unfolding get_memory_def contains_def separating_conjunction_def union_def disjoint_def
-  by (cases "m a"; auto)
-
-lemma "(((a \<mapsto> v) * (b \<mapsto> x)) * (c \<mapsto> y)) m \<Longrightarrow> get_memory a (state r m) = Some v"
-  unfolding get_memory_def contains_def separating_conjunction_def union_def disjoint_def
-  by force
+lemma load_wp_intro[THEN consequence, wp_intro]:
+  assumes "register_\<alpha> s pointer = Some (addr a)" "memory_\<alpha> s a = Some (Some v)"
+  shows "wp (execute_load name pointer s) (\<lambda>s'. memory_\<alpha> s' = memory_\<alpha> s \<and> register_\<alpha> s' = (register_\<alpha> s)(reg name := Some v))"
+  unfolding execute_load_def
+  using assms
+  apply simp
+  by (intro wp_intro; auto)
 
 
-lemma "((valid a) * B) m \<Longrightarrow> set_memory a v (state r m) \<noteq> None"
-  unfolding set_memory_def separating_conjunction_def union_def disjoint_def valid_def apply (cases "m a"; auto)
-  subgoal for mv apply (cases mv) apply auto by fastforce
-  done
+section "Add instruction"
+(* TODO: support pointers *)
+
+fun unsigned_overflow32 :: "word32 \<Rightarrow> word32 \<Rightarrow> bool" where
+  "unsigned_overflow32 a b = (a + b < a)"
+
+fun signed_overflow32 :: "word32 \<Rightarrow> word32 \<Rightarrow> bool" where
+  "signed_overflow32 a b = ((a <s 0 \<and> b <s 0 \<and> 0 \<le>s a+b) \<or> (0 \<le>s a \<and> 0 \<le>s b \<and> a+b <s 0))"
+
+(* a and b are negative \<longrightarrow> a + b must be negative *)
+(* a and b are positive \<longrightarrow> a + b must be positive *)
+(* a and b are different \<longrightarrow> a + b cannot overflow*)
+
+fun unsigned_overflow64 :: "word64 \<Rightarrow> word64 \<Rightarrow> bool" where
+  "unsigned_overflow64 a b = (a + b < a)"
+
+fun signed_overflow64 :: "word64 \<Rightarrow> word64 \<Rightarrow> bool" where
+  "signed_overflow64 a b = ((a <s 0 \<and> b <s 0 \<and> 0 \<le>s a+b) \<or> (0 \<le>s a \<and> 0 \<le>s b \<and> a+b <s 0))"
+
+definition add_no_poison32 :: "llvm_add_wrap \<Rightarrow> word32 \<Rightarrow> word32 \<Rightarrow> bool" where
+  "add_no_poison32 wrap a b = (
+      let uov = unsigned_overflow32 a b;
+          sov = signed_overflow32 a b
+      in case wrap of
+           add_default \<Rightarrow> True
+         | add_nuw \<Rightarrow> \<not>uov
+         | add_nsw \<Rightarrow> \<not>sov
+         | add_nuw_nsw \<Rightarrow> \<not>uov \<and> \<not>sov
+     )"
+
+declare add_no_poison32_def[simp]
+
+definition add_no_poison64 :: "llvm_add_wrap \<Rightarrow> word64 \<Rightarrow> word64 \<Rightarrow> bool" where
+  "add_no_poison64 wrap a b = (
+      let uov = unsigned_overflow64 a b;
+          sov = signed_overflow64 a b
+      in case wrap of
+           add_default \<Rightarrow> True
+         | add_nuw \<Rightarrow> \<not>uov
+         | add_nsw \<Rightarrow> \<not>sov
+         | add_nuw_nsw \<Rightarrow> \<not>uov \<and> \<not>sov
+     )"
+
+declare add_no_poison64_def[simp]
 
 
-lemma "((valid a) * B) m \<Longrightarrow> set_memory a v (state r m) = Some (state r' m') \<Longrightarrow> r' = r \<and> ((valid a) * B) m' \<and> ((a \<mapsto> v) * B) m'"
-  unfolding set_memory_def contains_def separating_conjunction_def valid_def disjoint_def union_def apply (intro conjI)
-    apply (cases "m a") apply simp apply simp subgoal for mv by (cases mv; simp)
-    apply (cases "m a") apply simp apply simp subgoal for mv apply (cases mv; simp)
-    apply (metis (no_types, lifting) dom_eq_singleton_conv fun_upd_upd insert_disjoint(2) map_add_upd_left map_upd_eqD1
-        memory_entry.distinct(6))
-    by (smt (verit) dom_empty dom_fun_upd fun_upd_None_if_notin_dom fun_upd_upd insert_disjoint(2) map_add_upd
-        map_add_upd_left map_upd_eqD1 memory_entry.distinct(6))
-    apply (cases "m a") apply simp apply simp subgoal for mv apply (cases mv; simp)
-     apply (metis dom_eq_singleton_conv fun_upd_upd insert_disjoint(2) map_add_upd_left)
-    apply auto
-    by (metis domIff dom_eq_singleton_conv fun_upd_upd map_add_upd_left)
-  done
+fun add_values :: "llvm_add_wrap \<Rightarrow> llvm_value \<Rightarrow> llvm_value \<Rightarrow> llvm_value option" where
+  "add_values wrap (vi32 a) (vi32 b) = (if add_no_poison32 wrap a b then Some (vi32 (a+b)) else Some poison)"
+| "add_values wrap (vi64 a) (vi64 b) = (if add_no_poison64 wrap a b then Some (vi64 (a+b)) else Some poison)"
+| "add_values _ poison (vi32 _) = Some poison"
+| "add_values _ (vi32 _) poison = Some poison"
+| "add_values _ poison (vi64 _) = Some poison"
+| "add_values _ (vi64 _) poison = Some poison"
+| "add_values _ poison poison = Some poison"
+| "add_values _ _ _ = None"
+
+
+definition execute_add :: "llvm_identifier \<Rightarrow> llvm_add_wrap \<Rightarrow> llvm_value_ref \<Rightarrow> llvm_value_ref \<Rightarrow> state \<Rightarrow> state option" where
+  "execute_add name wrap v1 v2 s = do {
+    v1' \<leftarrow> get_register s v1;
+    v2' \<leftarrow> get_register s v2;
+    res \<leftarrow> add_values wrap v1' v2';
+    set_register name res s
+  }"
+
+
+lemma add32_wp_intro[THEN consequence, wp_intro]:
+  assumes "register_\<alpha> s v1 = Some (vi32 v1')" "register_\<alpha> s v2 = Some (vi32 v2')" "add_no_poison32 wrap v1' v2'"
+  shows "wp (execute_add name wrap v1 v2 s) (\<lambda>s'. memory_\<alpha> s' = memory_\<alpha> s \<and> register_\<alpha> s' = (register_\<alpha> s)(reg name := Some (vi32 (v1' + v2'))))"
+  using assms
+  unfolding execute_add_def
+  by (intro wp_intro; simp; auto; intro wp_intro; simp)
+
+lemma add64_wp_intro[THEN consequence, wp_intro]:
+  assumes "register_\<alpha> s v1 = Some (vi64 v1')" "register_\<alpha> s v2 = Some (vi64 v2')" "add_no_poison64 wrap v1' v2'"
+  shows "wp (execute_add name wrap v1 v2 s) (\<lambda>s'. memory_\<alpha> s' = memory_\<alpha> s \<and> register_\<alpha> s' = (register_\<alpha> s)(reg name := Some (vi64 (v1' + v2'))))"
+  using assms
+  unfolding execute_add_def
+  by (intro wp_intro; simp; auto; intro wp_intro; simp)
 
 
 
-lemma allocate_heap_sep:
-  assumes "finite (dom h)"
-  assumes "(state r' h', a) = allocate_heap (state r h)"
-  shows "((\<lambda>h1. h1 = h) * (\<lambda>h2. h2 = [a \<mapsto> mem_unset])) h'"
-  unfolding separating_conjunction_def using assms unfolding allocate_stack_def apply auto
-  apply (metis (mono_tags, lifting) Int_insert_right_if0 allocate_heap_def disjoint_def dom_empty dom_fun_upd
-      fresh_heap_not_in_dom inf_bot_right option.distinct(1) snd_conv state.case)
-  by (metis (mono_tags, lifting) allocate_heap_def map_add_empty map_add_upd old.prod.inject state.case state.inject
-      union_def)
+section "Compare instruction"
+
+fun compare_values_32 :: "llvm_compare_condition \<Rightarrow> word32 \<Rightarrow> word32 \<Rightarrow> llvm_value" where
+  "compare_values_32 comp_eq a b = vi1 (a = b)"
+| "compare_values_32 comp_ne a b = vi1 (a \<noteq> b)"
+| "compare_values_32 comp_ugt a b = vi1 (a > b)"
+| "compare_values_32 comp_uge a b = vi1 (a \<ge> b)"
+| "compare_values_32 comp_ult a b = vi1 (a < b)"
+| "compare_values_32 comp_ule a b = vi1 (a \<le> b)"
+| "compare_values_32 comp_sgt a b = vi1 (b <s a)"
+| "compare_values_32 comp_sge a b = vi1 (b \<le>s a)"
+| "compare_values_32 comp_slt a b = vi1 (a <s b)"
+| "compare_values_32 comp_sle a b = vi1 (a \<le>s b)"
+
+fun compare_values_64 :: "llvm_compare_condition \<Rightarrow> word64 \<Rightarrow> word64 \<Rightarrow> llvm_value" where
+  "compare_values_64 comp_eq a b = vi1 (a = b)"
+| "compare_values_64 comp_ne a b = vi1 (a \<noteq> b)"
+| "compare_values_64 comp_ugt a b = vi1 (a > b)"
+| "compare_values_64 comp_uge a b = vi1 (a \<ge> b)"
+| "compare_values_64 comp_ult a b = vi1 (a < b)"
+| "compare_values_64 comp_ule a b = vi1 (a \<le> b)"
+| "compare_values_64 comp_sgt a b = vi1 (b <s a)"
+| "compare_values_64 comp_sge a b = vi1 (b \<le>s a)"
+| "compare_values_64 comp_slt a b = vi1 (a <s b)"
+| "compare_values_64 comp_sle a b = vi1 (a \<le>s b)"
+
+(* TODO: support pointers *)
+fun compare_values :: "llvm_compare_condition \<Rightarrow> llvm_value \<Rightarrow> llvm_value \<Rightarrow> llvm_value option" where
+  "compare_values c (vi32 a) (vi32 b) = Some (compare_values_32 c a b)"
+| "compare_values c (vi64 a) (vi64 b) = Some (compare_values_64 c a b)"
+| "compare_values _ _ _ = None"
+
+fun same_signs32 :: "word32 \<Rightarrow> word32 \<Rightarrow> bool" where
+  "same_signs32 a b = ((a <s 0 \<and> b <s 0) \<or> (0 \<le>s a \<and> 0 \<le>s b))"
+fun same_signs64 :: "word64 \<Rightarrow> word64 \<Rightarrow> bool" where
+  "same_signs64 a b = ((a <s 0 \<and> b <s 0) \<or> (0 \<le>s a \<and> 0 \<le>s b))"
+
+fun compare_values_sign :: "llvm_same_sign \<Rightarrow> llvm_compare_condition \<Rightarrow> llvm_value \<Rightarrow> llvm_value \<Rightarrow> llvm_value option" where
+  "compare_values_sign False c a b = compare_values c a b"
+| "compare_values_sign True c (vi32 a) (vi32 b) = (if same_signs32 a b then compare_values c (vi32 a) (vi32 b) else Some poison)"
+| "compare_values_sign True c (vi64 a) (vi64 b) = (if same_signs64 a b then compare_values c (vi64 a) (vi64 b) else Some poison)"
+| "compare_values_sign True c _ _ = None"
+
+definition execute_icmp :: "llvm_identifier \<Rightarrow> llvm_same_sign \<Rightarrow> llvm_compare_condition \<Rightarrow> llvm_value_ref \<Rightarrow> llvm_value_ref \<Rightarrow> state \<Rightarrow> state option" where
+  "execute_icmp name same_sign cond v1 v2 s = do {
+    v1' \<leftarrow> get_register s v1;
+    v2' \<leftarrow> get_register s v2;
+    res \<leftarrow> compare_values_sign same_sign cond v1' v2';
+    set_register name res s
+  }"
+
+lemma icmp32_wp_intro[THEN consequence, wp_intro]:
+  assumes "register_\<alpha> s v1 = Some (vi32 v1')" "register_\<alpha> s v2 = Some (vi32 v2')" "(if ss then same_signs32 v1' v2' else True)"
+  shows "wp (execute_icmp name ss cond v1 v2 s) (\<lambda>s'. memory_\<alpha> s' = memory_\<alpha> s \<and> register_\<alpha> s' = (register_\<alpha> s)(reg name := Some (compare_values_32 cond v1' v2')))"
+  using assms
+  unfolding execute_icmp_def
+  by (cases ss; intro wp_intro; auto; intro wp_intro; auto)
+
+lemma icmp64_wp_intro[THEN consequence, wp_intro]:
+  assumes "register_\<alpha> s v1 = Some (vi64 v1')" "register_\<alpha> s v2 = Some (vi64 v2')" "(if ss then same_signs64 v1' v2' else True)"
+  shows "wp (execute_icmp name ss cond v1 v2 s) (\<lambda>s'. memory_\<alpha> s' = memory_\<alpha> s \<and> register_\<alpha> s' = (register_\<alpha> s)(reg name := Some (compare_values_64 cond v1' v2')))"
+  using assms
+  unfolding execute_icmp_def
+  by (cases ss; intro wp_intro; auto; intro wp_intro; auto)
+
+
+
+section "Phi nodes"
+
+fun phi_lookup :: "llvm_identifier option \<Rightarrow> (llvm_identifier * llvm_value_ref) list \<Rightarrow> llvm_value_ref option" where
+  "phi_lookup l ls = do {
+    prev \<leftarrow> l;
+    assert (distinct (map fst ls));
+    map_of ls prev
+  }"
+
+definition execute_phi :: "llvm_phi_node \<Rightarrow> llvm_identifier option \<Rightarrow> state \<Rightarrow> state option" where
+  "execute_phi p prev s =
+    (case p of (phi name type values) \<Rightarrow>
+      do {
+        v \<leftarrow> phi_lookup prev values;
+        v' \<leftarrow> get_register s v;
+        set_register name v' s
+      }
+    )"
+
+
+section "Blocks and functions"
+
+context
+  fixes program :: llvm_program
+begin
+
+datatype exec_type = exec_instruction llvm_instruction
+  | exec_block "llvm_identifier option" llvm_instruction_block
+  | exec_blocks "llvm_identifier option" llvm_identifier llvm_labeled_blocks
+  | exec_func "llvm_identifier" "llvm_value list"
+
+datatype exec_result = state_only state
+  | ctrl_flow state llvm_block_return
+  | func_ret state "llvm_value option"
+
+
+fun stack_size :: "state \<Rightarrow> nat" where
+  "stack_size (state l g s h) = length s"
+fun restore_stack :: "state \<Rightarrow> nat \<Rightarrow> state" where
+  "restore_stack (state l g s h) n = (state l g (take n s) h)"
+fun local_registers :: "state \<Rightarrow> (llvm_register_model * state)" where
+  "local_registers (state l g s h) = (l, (state Mapping.empty g s h))"
+fun restore_registers :: "state \<Rightarrow> llvm_register_model \<Rightarrow> state" where
+  "restore_registers (state _ g s h) l = (state l g s h)"
+
+fun store_parameters :: "llvm_identifier list \<Rightarrow> llvm_value list \<Rightarrow> state \<Rightarrow> state option" where
+  "store_parameters (i#is) (v#vs) s = do {
+    s' \<leftarrow> set_register i v s;
+    store_parameters is vs s'
+  }"
+| "store_parameters [] [] s = Some s"
+| "store_parameters _ _ _ = None"
+
+fun get_parameters :: "llvm_value_ref list \<Rightarrow> state \<Rightarrow> (llvm_value list) option" where
+  "get_parameters (v#vs) s = do {
+    v' \<leftarrow> get_register s v;
+    vs' \<leftarrow> get_parameters vs s;
+    Some (v'#vs')
+  }"
+| "get_parameters [] _ = Some []"
+
+
+partial_function (option) exec where
+  "exec t s = (case t of
+    exec_instruction (call name type fun pars) \<Rightarrow>
+      do {
+        ps \<leftarrow> get_parameters (map snd pars) s;
+        ret \<leftarrow> exec (exec_func fun ps) s;
+        (s', v) \<leftarrow> (case ret of
+          func_ret s' v \<Rightarrow> Some (s', v)
+        | _ \<Rightarrow> None);
+        s'' \<leftarrow>
+          (case name of
+            Some n \<Rightarrow> do {
+              v' \<leftarrow> v;
+              set_register n v' s'
+            }
+          | None \<Rightarrow> Some s'
+          );
+        Some (state_only s'')
+      }
+  | exec_instruction i \<Rightarrow>
+      do {
+        s' \<leftarrow> (case i of
+          alloca name type align              \<Rightarrow> execute_alloca name s
+        | store type value pointer align      \<Rightarrow> execute_store value pointer s
+        | load name type pointer align        \<Rightarrow> execute_load name pointer s
+        | add name wrap type v1 v2            \<Rightarrow> execute_add name wrap v1 v2 s
+        | icmp name same_sign cond type v1 v2 \<Rightarrow> execute_icmp name same_sign cond v1 v2 s
+        );
+        Some (state_only s')
+      }
+  | exec_block prev b \<Rightarrow>
+    (case b of
+      (p#ps,is,t) \<Rightarrow> do {
+        s' \<leftarrow> execute_phi p prev s;
+        exec (exec_block prev (ps,is,t)) s'
+      }
+    | ([],i#is,t) \<Rightarrow> do {
+        s' \<leftarrow> exec (exec_instruction i) s;
+        (case s' of
+          state_only s' \<Rightarrow> exec (exec_block prev ([],is,t)) s'
+        | _ \<Rightarrow> None
+        )
+      }
+    | ([],[],t) \<Rightarrow>
+      (case t of
+        ret r \<Rightarrow>
+          (case r of
+            Some (t, v) \<Rightarrow>
+              (case get_register s v of
+                Some v' \<Rightarrow> Some (ctrl_flow s (return_value (Some v')))
+              | _     \<Rightarrow> None
+              )
+          | None \<Rightarrow> Some (ctrl_flow s (return_value None))
+          )
+      | br_i1 b l1 l2 \<Rightarrow>
+          (case get_register s b of
+            Some (vi1 b') \<Rightarrow> Some (ctrl_flow s (branch_label (if b' then l1 else l2)))
+          | _           \<Rightarrow> None
+          )
+      | br_label l \<Rightarrow> Some (ctrl_flow s (branch_label l))
+      )
+    )
+  | exec_blocks pre cur lbs \<Rightarrow>
+      do {
+        block \<leftarrow> map_of lbs cur;
+        s' \<leftarrow> exec (exec_block pre block) s;
+        (case s' of
+          ctrl_flow s' br \<Rightarrow>
+            (case br of
+              branch_label l \<Rightarrow> exec (exec_blocks (Some cur) l lbs) s'
+            | return_value v \<Rightarrow> Some (func_ret s' v)
+            )
+        | _ \<Rightarrow> None
+        )
+      }
+  | exec_func name pars \<Rightarrow>
+    do { \<comment> \<open>store initial state that needs to be restored (stack, local registers) \<close>
+      (l, s') \<leftarrow> Some (local_registers s);
+      stack_len \<leftarrow> Some (stack_size s);
+      f  \<leftarrow> map_of (funcs program) name;
+      fb \<leftarrow>
+        (case llvm_function.blocks f of
+          ((fb,_)#_) \<Rightarrow> Some fb
+        | _ \<Rightarrow> None
+        );
+      ret \<leftarrow> exec (exec_blocks None fb (llvm_function.blocks f)) s';
+      (s'', v) \<leftarrow>
+        (case ret of
+          func_ret s v \<Rightarrow> Some (s, v)
+        | _ \<Rightarrow> None
+        );
+      Some (func_ret (restore_stack (restore_registers s'' l) stack_len) v)
+    }
+  )"
+
+end
+
+partial_function (option)
+  execute_instruction :: "llvm_instruction \<Rightarrow> state \<Rightarrow> exec_Some option"
+where
+  "execute_instruction ii is = (case (case ii of
+    \<comment> \<open>Allocate new memory value on the stack, and set the specified register to its address\<close>
+    alloca name type align              \<Rightarrow> execute_alloca name is
+    \<comment> \<open>Read address from pointer and store value in the stack or the heap\<close>
+  | store type value pointer align      \<Rightarrow> execute_store value pointer is
+    \<comment> \<open>Read address from pointer and load value from either the stack or the heap\<close>
+  | load name type pointer align        \<Rightarrow> execute_load name pointer is
+    \<comment> \<open>Get values, add according to wrap option (or poison), and store in register\<close>
+  | add name wrap type v1 v2            \<Rightarrow> execute_add name wrap v1 v2 is
+    \<comment> \<open>Get values, do comparison, and store in register\<close>
+  | icmp name same_sign cond type v1 v2 \<Rightarrow> execute_icmp name same_sign cond v1 v2 is
+  ) of Some s' \<Rightarrow> Some (state_only s') | _ \<Rightarrow> None)"
+
+partial_function (option)
+  execute_block :: "llvm_identifier option \<Rightarrow> llvm_instruction_block \<Rightarrow> state \<Rightarrow> exec_result option"
+  where
+ "execute_block previous bb bs = (case bb of
+    ((phi name type values)#ps, is, t) \<Rightarrow>
+    (case execute_phi previous name values bs of
+      Some s' \<Rightarrow> execute_block previous (ps, is, t) s'
+    | err e \<Rightarrow> None
+    )
+  | (_, i#is, t) \<Rightarrow>
+    (case execute_instruction i bs of
+      Some (state_only s') \<Rightarrow> execute_block previous ([],is,t) s'
+    | _ \<Rightarrow> None
+    )
+  | (_, _, br_i1 v l1 l2) \<Rightarrow>
+    (case (do {
+      val \<leftarrow> get_register bs v;
+      label \<leftarrow> (case val of (vi1 b) \<Rightarrow> Some (if b then l1 else l2) | _ \<Rightarrow> err incompatible_types);
+      Some (ctrl_flow bs (branch_label label))
+    }) of Some x \<Rightarrow> Some x | _ \<Rightarrow> None)
+  | (_, _, br_label l) \<Rightarrow>
+    Some (ctrl_flow bs (branch_label l))
+  | (_, _, ret t v) \<Rightarrow>
+    (case get_register bs v of
+      Some v' \<Rightarrow> Some (ctrl_flow bs (return_value v'))
+    | _ \<Rightarrow> None
+    )
+  )"
+
+partial_function (tailrec)
+  execute_blocks :: "llvm_identifier option \<Rightarrow> llvm_identifier \<Rightarrow> llvm_labeled_blocks \<Rightarrow> state \<Rightarrow> exec_Some option"
+where
+ "execute_blocks bsp bsl bsb bss =
+    (case map_of bsb bsl of
+      None \<Rightarrow> err unknown_label
+    | Some block \<Rightarrow>
+      (case execute_block bsp block bss of
+        err e \<Rightarrow> err e
+      | Some (ctrl_flow s' br) \<Rightarrow>
+        (case br of
+          return_value v \<Rightarrow> Some (func_ret s' (Some v))
+        | branch_label l \<Rightarrow> execute_blocks (Some bsl) l bsb s'
+        )
+      | _ \<Rightarrow> err internal_error
+      )
+    )"
+
+partial_function (tailrec) execute_function :: "llvm_function \<Rightarrow> state \<Rightarrow> (state * llvm_value option) option" where
+  "execute_function (func _ ((l,b)#ls)) s = execute_blocks None l ((l,b)#ls) s"
+| "execute_function _ s = Some (s, None)"
+
+
+
+lemmas [code] = execute_blocks.simps
+
+
+
+section "Intro Rules"
+
+lemma [wp_intro]: "wp (execute_alloca name s) Q \<Longrightarrow> wp (execute_instruction (alloca name type align) s) Q"
+  by (simp add: execute_instruction.simps)
+lemma [wp_intro]: "wp (execute_store value pointer s) Q \<Longrightarrow> wp (execute_instruction (store type value pointer align) s) Q"
+  by (simp add: execute_instruction.simps)
+lemma [wp_intro]: "wp (execute_load name pointer s) Q \<Longrightarrow> wp (execute_instruction (load name type pointer align) s) Q"
+  by (simp add: execute_instruction.simps)
+lemma [wp_intro]: "wp (execute_add name wrap v1 v2 s) Q \<Longrightarrow> wp (execute_instruction (add name wrap type v1 v2) s) Q"
+  by (simp add: execute_instruction.simps)
+lemma [wp_intro]: "wp (execute_icmp name same_sign cond v1 v2 s) Q \<Longrightarrow> wp (execute_instruction (icmp name same_sign cond type v1 v2) s) Q"
+  by (simp add: execute_instruction.simps)
+
+
+lemma block_phi_wp_intro[wp_intro]:
+  assumes "wp (execute_phi p name values s) (\<lambda>s'. wp (execute_block p (ps, is, t) s') Q)"
+  shows "wp (execute_block p ((phi name type values)#ps, is, t) s) Q"
+  apply (subst execute_block.simps)
+  using assms
+  unfolding wp_gen_def
+  by (auto split: option.splits list.splits)
+
+lemma block_instr_wp_intro[wp_intro]:
+  assumes "wp (execute_instruction i s) (\<lambda>s'. wp (execute_block p ([], is, t) s') Q)"
+  shows "wp (execute_block p ([], i#is, t) s) Q"
+  apply (subst execute_block.simps)
+  using assms
+  unfolding wp_gen_def
+  by (auto split: option.splits)
+
+lemma block_ret_wp_intro[THEN consequence, wp_intro]:
+  assumes "register_\<alpha> s value = Some v"
+  shows "wp (execute_block p ([], [], ret type value) s) (\<lambda>r. r = (s, return_value v))"
+  apply (subst execute_block.simps)
+  using assms
+  unfolding wp_gen_def
+  apply (cases s; cases "value")
+  by (auto simp: return_def split: option.splits)
+
+lemma block_br_label_wp_intro[THEN consequence, wp_intro]:
+  shows "wp (execute_block p ([], [], br_label l) s) (\<lambda>r. r = (s, branch_label l))"
+  apply (subst execute_block.simps)
+  unfolding wp_gen_def
+  by (auto simp: return_def)
+
+lemma block_br_i1_wp_intro[THEN consequence, wp_intro]:
+  assumes "register_\<alpha> s value = Some (vi1 b)"
+  shows "wp (execute_block p ([], [], br_i1 value l1 l2) s) (\<lambda>r. r = (s, branch_label (if b then l1 else l2)))"
+  apply (subst execute_block.simps)
+  unfolding wp_gen_def
+  using assms
+  by (auto simp: return_def split: option.splits)
+
+lemma phi_wp_intro[THEN consequence, wp_intro]:
+  assumes "distinct (map fst values)"
+  assumes "p = Some p'" "map_of values p' = Some v" "register_\<alpha> s v = Some v'"
+  shows "wp (execute_phi p name values s) (\<lambda>s'. register_\<alpha> s' = (register_\<alpha> s)(reg name := Some v') \<and> memory_\<alpha> s' = memory_\<alpha> s)"
+  unfolding execute_phi_def
+  apply simp
+  using assms
+  apply (intro wp_intro; auto) done
 
 end
