Registers.thy
@@ -4,21 +4,21 @@ begin
 
 section "Simps"
 
-lemma memory_\<alpha>_eq[simp]: "memory_\<alpha> (l,g,s,h) = memory_\<alpha> (l',g',s,h)"
+lemma memory_\<alpha>_eq[simp]: "memory_\<alpha> (state l g s h) = memory_\<alpha> (state l' g' s h)"
   apply (rule ext)
   subgoal for x
     by (cases x; simp)
   done
 
 lemma register_\<alpha>_lid_update_eq[simp]:
-  "register_\<alpha> (Mapping.update n v l, g, s, h) = (register_\<alpha> (l, g, s, h))(reg (lid n) := Some v)"
+  "register_\<alpha> (state (Mapping.update n v l) g s h) = (register_\<alpha> (state l g s h))(reg (lid n) := Some v)"
   apply (auto simp: fun_eq_iff split: llvm_value_ref.split)
   subgoal for x apply (cases x; simp) subgoal for id by (cases id; simp)
   done
   done
 
 lemma register_\<alpha>_gid_update_eq[simp]:
-  "register_\<alpha> (l, Mapping.update n v g, s, h) = (register_\<alpha> (l, g, s, h))(reg (gid n) := Some v)"
+  "register_\<alpha> (state l (Mapping.update n v g) s h) = (register_\<alpha> (state l g s h))(reg (gid n) := Some v)"
   apply (auto simp: fun_eq_iff split: llvm_value_ref.split)
   subgoal for x apply (cases x; simp) subgoal for id by (cases id; simp)
   done
@@ -33,41 +33,38 @@ lemma register_\<alpha>_update_independent[simp]:
   by (metis fun_upd_other)
 
 
-
-section "register_\<alpha> operation"
-
-lemma set_register_\<alpha>:
-  "register_\<alpha> (set_register n v s) = (register_\<alpha> s)(reg n := Some v)"
-  apply (cases s; rule ext)
-  subgoal for l' g' s' h' x by (cases x; cases n; auto simp: set_single_register_def)
+lemma register_\<alpha>_eq_get_register[simp]:
+  "register_\<alpha> s r = get_register s r"
+  apply (cases s; cases r; auto)
+  subgoal for _ _ _ _ i
+    by (cases i; simp)
   done
-
 
 
 section "Intro rules"
 
-named_theorems register_intro
+named_theorems single_register_intro
 
-lemma wp_set_single_register_lid_intro[THEN consequence, register_intro]:
-  "wp (return (set_single_register n v l,g,s,h)) (\<lambda>s'. register_\<alpha> s' = (register_\<alpha> (l,g,s,h))(reg (lid n) := Some v) \<and> memory_\<alpha> s' = memory_\<alpha> (l,g,s,h))"
+lemma wp_set_single_register_lid_intro[THEN consequence, single_register_intro]:
+  "wp (Some (state (set_single_register n v l) g s h)) (\<lambda>s'. register_\<alpha> s' = (register_\<alpha> (state l g s h))(reg (lid n) := Some v) \<and> memory_\<alpha> s' = memory_\<alpha> (state l g s h))"
   unfolding set_single_register_def
-  by (intro wp_intro wp_return_intro; simp)
+  by (intro wp_intro; simp)
 
-lemma wp_set_single_register_gid_intro[THEN consequence, register_intro]:
-  "wp (return (l,set_single_register n v g,s,h)) (\<lambda>s'. register_\<alpha> s' = (register_\<alpha> (l,g,s,h))(reg (gid n) := Some v) \<and> memory_\<alpha> s' = memory_\<alpha> (l,g,s,h))"
+lemma wp_set_single_register_gid_intro[THEN consequence, single_register_intro]:
+  "wp (Some (state l (set_single_register n v g) s h)) (\<lambda>s'. register_\<alpha> s' = (register_\<alpha> (state l g s h))(reg (gid n) := Some v) \<and> memory_\<alpha> s' = memory_\<alpha> (state l g s h))"
   unfolding set_single_register_def
-  by (intro wp_intro wp_return_intro; simp)
+  by (intro wp_intro; simp)
 
 lemma wp_set_register_intro[THEN consequence, wp_intro]:
-  shows "wp (return (set_register n v s)) (\<lambda>s'. register_\<alpha> s' = (register_\<alpha> s)(reg n := Some v) \<and> memory_\<alpha> s' = memory_\<alpha> s)"
-  by (cases n; cases s; simp; intro wp_intro register_intro; simp)
+  shows "wp (set_register n v s) (\<lambda>s'. register_\<alpha> s' = (register_\<alpha> s)(reg n := Some v) \<and> memory_\<alpha> s' = memory_\<alpha> s)"
+  by (cases n; cases s; simp; intro wp_intro single_register_intro; simp)
 
 
 lemma wp_get_register_intro[THEN consequence, wp_intro]:        
   assumes "register_\<alpha> s n \<noteq> None"
   shows "wp (get_register s n) (\<lambda>v'. register_\<alpha> s n = Some v')"
   using assms
-  apply (cases s; cases n) subgoal for _ _ _ _ id by (cases id; simp; intro wp_intro; auto)
-  by simp
+  unfolding wp_def
+  by auto
 
 end
