WeakestPreconditions.thy
@@ -1,0 +1,97 @@
+theory WeakestPreconditions
+  imports "HOL-Library.Monad_Syntax"
+begin
+
+section "Definitions"
+                   
+fun assert where "assert True = Some ()" | "assert False = None"
+
+definition wp :: "'a option \<Rightarrow> ('a \<Rightarrow> bool) \<Rightarrow> bool" where
+  "wp m P = (case m of Some v \<Rightarrow> P v | None \<Rightarrow> False)"
+
+
+
+section "Lemmas"
+
+named_theorems wp_intro
+
+subsection "Assert simps"
+
+lemma assert_simps[simp]:            
+  "assert P = Some x \<longleftrightarrow> P"
+  "assert P = None \<longleftrightarrow> \<not>P"
+  using assert.elims
+  by auto
+
+
+subsection "Intro rules"
+
+context
+  notes wp_def[simp]
+begin
+
+lemma consequence:
+  assumes "wp x Q"
+  assumes "\<And>x. Q x \<Longrightarrow> Q' x"
+  shows "wp x Q'"
+  using assms
+  by (cases x; simp)
+
+
+lemma wp_Some_intro[wp_intro, simp]:
+  assumes "Q x"
+  shows "wp (Some x) Q"
+  using assms
+  by simp
+
+lemma wp_None_intro[wp_intro, simp]:
+  shows "\<not>wp (None) Q"
+  by simp
+
+
+lemma wp_assert_intro[wp_intro]:
+  assumes "b"
+  assumes "b \<Longrightarrow> wp f P"
+  shows "wp (do {assert b; f}) P"
+  using assms
+  by (cases b; simp)
+
+
+lemma wp_bind_intro[wp_intro]:
+  assumes "wp m (\<lambda>x. wp (f x) P)"
+  shows "wp (do {x\<leftarrow>m; f x}) P"
+  using assms
+  by (cases m; simp add: bind_def)
+
+
+lemma wp_case_option_intro[wp_intro]:
+  assumes "c = None \<Longrightarrow> wp f P"
+  assumes "\<And>v. c = Some v \<Longrightarrow> wp (g v) P"
+  shows "wp (case c of None \<Rightarrow> f | Some v \<Rightarrow> g v) P"
+  using assms
+  by (cases c; simp)
+
+
+lemma wp_if_intro[wp_intro]:
+  assumes "b \<Longrightarrow> wp T Q"
+  assumes "\<not>b \<Longrightarrow> wp F Q"
+  shows "wp (if b then T else F) Q"
+  using assms
+  by auto
+
+lemma wp_case_product_intro[wp_intro]:
+  assumes "\<And>b c. a = (b,c) \<Longrightarrow> wp (f b c) Q"
+  shows "wp (case a of (b,c) \<Rightarrow> f b c) Q"
+  using assms
+  by (cases a; simp)
+
+lemma wp_option_intro:
+  assumes "f \<noteq> None"
+  assumes "\<And>x. f = Some x \<Longrightarrow> Q x"
+  shows "wp f Q"
+  using assms
+  by auto
+
+end
+
+end
